

# The Poisson summation formula

Henry Twiss

## 1 The Fourier Transform

Let  $f(\mathbf{x})$  be absolutely integrable on  $\mathbb{R}^n$ . Its *Fourier transform*  $(\mathcal{F}f)(\boldsymbol{\xi})$  is defined by

$$(\mathcal{F}f)(\boldsymbol{\xi}) = \int_{\mathbb{R}^n} f(\mathbf{x}) e^{-2\pi i \langle \boldsymbol{\xi}, \mathbf{x} \rangle} d\mathbf{x},$$

for  $\boldsymbol{\xi} \in \mathbb{R}^n$ . It is absolutely bounded precisely because  $f(\mathbf{x})$  is absolutely integrable on  $\mathbb{R}^n$ . Let us first demonstrate some properties of the Fourier transform.

**Proposition 1.1.** *Let  $f(\mathbf{x})$  and  $g(\mathbf{x})$  be absolutely integrable on  $\mathbb{R}^n$ . Then the following properties hold:*

(i) *For any  $\alpha, \beta \in \mathbb{R}$ , we have*

$$(\mathcal{F}(\alpha f + \beta g))(\boldsymbol{\xi}) = \alpha(\mathcal{F}f)(\boldsymbol{\xi}) + \beta(\mathcal{F}g)(\boldsymbol{\xi}).$$

(ii) *If  $g(\mathbf{x}) = f(\mathbf{x} + \boldsymbol{\alpha})$  for any  $\boldsymbol{\alpha} \in \mathbb{R}^n$  then*

$$(\mathcal{F}g)(\boldsymbol{\xi}) = e^{2\pi i \langle \boldsymbol{\alpha}, \boldsymbol{\xi} \rangle} (\mathcal{F}f)(\boldsymbol{\xi}).$$

(iii) *If  $g(\mathbf{x}) = f(A\mathbf{x})$  for any  $A \in \text{GL}_n(\mathbb{R})$  then*

$$(\mathcal{F}g)(\boldsymbol{\xi}) = \frac{1}{|\det(A)|} (\mathcal{F}f)((A^{-1})^t \boldsymbol{\xi}).$$

*Proof.* Property (i) is immediate from linearity of the integral while (ii) follows by applying the change of variables  $\mathbf{x} \mapsto \mathbf{x} - \boldsymbol{\alpha}$ . Property (iii) is proved by performing the change of variables  $\mathbf{x} \mapsto A^{-1}\mathbf{x}$  which has Jacobian matrix  $A^{-1}$  with Jacobian determinant  $\frac{1}{|\det(A)|}$ .  $\square$

## 2 Fourier Series

The Fourier transform is intimately related to periodic functions. Let  $\Lambda$  be a complete integral lattice in  $\mathbb{R}^n$  with fundamental domain  $\mathcal{M}$  and denote the dual lattice by  $\Lambda^\vee$ .

Suppose  $f(\mathbf{x})$  is  $\Lambda$ -periodic and integrable on  $\mathcal{M}$ . Then we define the  $\lambda^\vee$ -th *Fourier coefficient*  $\hat{f}(\lambda^\vee)$  of  $f(\mathbf{x})$  by

$$\hat{f}(\lambda^\vee) = \int_{\mathcal{M}} f(\mathbf{x}) e^{-2\pi i \langle \lambda^\vee, \mathbf{x} \rangle} d\mathbf{x}.$$

The *Fourier series*  $S_f(x)$  is defined by

$$S_f(\mathbf{x}) = \frac{1}{V_\Lambda} \sum_{\lambda^\vee \in \Lambda^\vee} \hat{f}(\lambda^\vee) e^{2\pi i \langle \lambda^\vee, \mathbf{x} \rangle}.$$

Notice that the Fourier coefficients are only defined for elements of the dual lattice and that the Fourier series is a sum over these elements. A crucial question is where the Fourier series of  $f(\mathbf{x})$  converges, if at all, and if so does it even converge to  $f(\mathbf{x})$  itself. Under quite reasonable conditions the Fourier series converges uniformly to the function itself, but we first make a reduction. Fix a basis  $\lambda_1, \dots, \lambda_n$  for  $\Lambda$  and let  $P$  be the associated generator matrix. This means  $P$  is the base change matrix from the standard basis to  $\lambda_1, \dots, \lambda_n$  so that  $P$  is the unique invertible linear transformation on  $\mathbb{R}^n$  satisfying  $\Lambda = P\mathbb{Z}^n$  and  $\Lambda^\vee = (P^{-1})^t\mathbb{Z}^n$ . Letting  $f_P(\mathbf{x}) = f(P\mathbf{x})$ , we see that  $f_P(\mathbf{x})$  is 1-periodic in each component and integrable on  $[0, 1]^n$ . As  $\mathbb{Z}^n$  is self-dual and its covolume is 1, the  $\mathbf{n}$ -th Fourier coefficient  $\hat{f}_P(\mathbf{n})$  of  $f_P(\mathbf{x})$  is given by

$$\hat{f}_P(\mathbf{n}) = \int_{[0,1]^n} f(\mathbf{x}) e^{-2\pi i \langle \mathbf{n}, \mathbf{x} \rangle} d\mathbf{x}.$$

and the Fourier series is

$$S_{f_P}(\mathbf{x}) = \sum_{\mathbf{n} \in \mathbb{Z}^n} \hat{f}_P(\mathbf{n}) e^{2\pi i \langle \mathbf{n}, \mathbf{x} \rangle}.$$

As  $P$  is invertible, it suffices to study the convergence properties of this Fourier series. The reduction here this that we may assume our Fourier series are 1-periodic in each component and in this case we have the following well-known result:

**Theorem 2.1.** *Suppose  $f(\mathbf{x})$  is a smooth function on  $\mathbb{R}^n$  and is 1-periodic in each component. Then the Fourier series of  $f(\mathbf{x})$  converges uniformly everywhere to  $f(\mathbf{x})$ .*

In the case of 1-periodic functions of a single variable, we can do better as we may merely assume  $f(x)$  is of bounded variation. This is known as the *Dirichlet-Jordan test*:

**Theorem (Dirichlet-Jordan test).** *Suppose  $f(x)$  is a function on  $\mathbb{R}$  which is 1-periodic and of bounded variation. Then the Fourier series of  $f(x)$  converges locally uniformly to  $f(x)$  on every set where  $f(x)$  is continuous. Moreover, at any jump discontinuity, the Fourier series of  $f(x)$  converges to the average of the left-hand and right-hand limits of  $f(x)$ . In particular, this holds for all continuously differentiable functions with at most a finite number of jump discontinuities.*

### 3 Poisson Summation

Returning to the general setting, there are two ways of building a function from  $f(\mathbf{x})$  that is  $\lambda$ -periodic. The first is to average  $f(\mathbf{x})$  over all translates by elements of  $\Lambda$  while the second is to considering its Fourier series  $f(\mathbf{x})$ . This gives us the two series

$$\sum_{\lambda \in \Lambda} f(\mathbf{x} + \lambda) \quad \text{or} \quad \frac{1}{V_\Lambda} \sum_{\lambda^\vee \in \Lambda^\vee} (\mathcal{F}f)(\lambda^\vee) e^{2\pi i \langle \lambda^\vee, \mathbf{x} \rangle}.$$

The link between the Fourier transform and Fourier series is given by the *Poisson summation formula* which says that these two expressions are the same under some mild assumptions.

**Theorem (Poisson summation formula).** *Suppose  $\Lambda$  is a complete integral lattice in  $\mathbb{R}^n$ ,  $f(\mathbf{x})$  is absolutely integrable on  $\mathbb{R}^n$ , and the function*

$$F(\mathbf{x}) = \sum_{\lambda \in \Lambda} f(\mathbf{x} + \lambda),$$

*is smooth. Then*

$$\sum_{\lambda \in \Lambda} f(\mathbf{x} + \lambda) = \frac{1}{V_\Lambda} \sum_{\lambda^\vee \in \Lambda^\vee} (\mathcal{F}f)(\lambda^\vee) e^{2\pi i \langle \lambda^\vee, \mathbf{x} \rangle},$$

*and*

$$\sum_{\lambda \in \Lambda} f(\lambda) = \frac{1}{V_\Lambda} \sum_{\lambda^\vee \in \Lambda^\vee} (\mathcal{F}f)(\lambda^\vee).$$

*Proof.* Fix a basis  $\lambda_1, \dots, \lambda_n$  for  $\Lambda$  and let  $P$  be the associated generator matrix. Then  $\Lambda = P\mathbb{Z}^n$  and  $\Lambda^\vee = (P^{-1})^t \mathbb{Z}^n$ . Letting  $F_P(\mathbf{x}) = F(P\mathbf{x})$ , we may write

$$F_P(\mathbf{x}) = \sum_{\mathbf{n} \in \mathbb{Z}^n} f(P\mathbf{x} + P\mathbf{n}).$$

$F_P(\mathbf{x})$  is smooth and 1-periodic in each component because  $F(\mathbf{x})$  is smooth and invariant under translation by  $\Lambda$ . Whence  $F_P(\mathbf{x})$  admits a Fourier series converging uniformly everywhere to  $F_P(\mathbf{x})$ . Moreover,  $F_P(\mathbf{x})$  is absolutely integrable on  $[0, 1]^n$ . We will compute the  $\mathbf{t}$ -th Fourier coefficient of  $F_P(\mathbf{x})$  given by

$$\hat{F}_P(\mathbf{t}) = \int_{[0,1]^n} F_P(\mathbf{x}) e^{-2\pi i \langle \mathbf{t}, \mathbf{x} \rangle} d\mathbf{x}$$

The absolute integrability of  $f(\mathbf{x})$  permits the interchange of sum and integral to obtain

$$\sum_{\mathbf{n} \in \mathbb{Z}^n} \int_{[0,1]^n} f(P\mathbf{x} + P\mathbf{n}) e^{-2\pi i \langle \mathbf{t}, \mathbf{x} \rangle} d\mathbf{x}.$$

The change of variables  $\mathbf{x} \mapsto P^{-1}\mathbf{x}$  gives

$$\frac{1}{V_\Lambda} \sum_{\mathbf{n} \in \mathbb{Z}^n} \int_{P[0,1]^n} f(\mathbf{x} + P\mathbf{n}) e^{-2\pi i \langle (P^{-1})^t \mathbf{t}, \mathbf{x} \rangle} d\mathbf{x},$$

because the Jacobian matrix is  $P^{-1}$  with Jacobian determinant  $\frac{1}{V_\Lambda}$ . This expression is simply

$$\frac{1}{V_\Lambda} \int_{\mathbb{R}^n} f(\mathbf{x}) e^{-2\pi i \langle (P^{-1})^t \mathbf{t}, \mathbf{x} \rangle} d\mathbf{x} = \frac{1}{V_\Lambda} (\mathcal{F}f)((P^{-1})^t \mathbf{t}).$$

Whence

$$\sum_{\lambda \in \Lambda} f(P\mathbf{x} + \lambda) = \frac{1}{V_\Lambda} \sum_{\mathbf{t} \in \mathbb{Z}^n} (\mathcal{F}f)((P^{-1})^t \mathbf{t}) e^{2\pi i \langle \mathbf{t}, \mathbf{x} \rangle}.$$

Changing variables  $\mathbf{x} \mapsto P^{-1}\mathbf{x}$  results in

$$\sum_{\lambda \in \Lambda} f(\mathbf{x} + \lambda) = \frac{1}{V_\Lambda} \sum_{\lambda^\vee \in \Lambda^\vee} (\mathcal{F}f)(\lambda^\vee) e^{2\pi i \langle \lambda^\vee, \mathbf{x} \rangle}.$$

This proves the first statement. Setting  $\mathbf{x} = \mathbf{0}$  proves the second statement.  $\square$

For convenience, we state the Poisson summation formula in the simplified case for the complete integral lattice  $\mathbb{Z}^n$  as a corollary since it is how the Poisson summation formula is usually applied.

**Corollary 3.1.** *Suppose  $f(\mathbf{x})$  is absolutely integrable on  $\mathbb{R}^n$ , and the function*

$$F(\mathbf{x}) = \sum_{\mathbf{n} \in \mathbb{Z}^n} f(\mathbf{x} + \mathbf{n}),$$

*is smooth. Then*

$$\sum_{\mathbf{n} \in \mathbb{Z}^n} f(\mathbf{x} + \mathbf{n}) = \sum_{\mathbf{t} \in \mathbb{Z}^n} (\mathcal{F}f)(\mathbf{t}) e^{2\pi i \langle \mathbf{t}, \mathbf{x} \rangle},$$

*and*

$$\sum_{\mathbf{n} \in \mathbb{Z}^n} f(\mathbf{n}) = \sum_{\mathbf{t} \in \mathbb{Z}^n} (\mathcal{F}f)(\mathbf{t}).$$

*Proof.* This is the Poisson summation formula for the complete integral lattice  $\mathbb{Z}^n$  since  $\mathbb{Z}^n$  is self-dual and  $V_{\mathbb{Z}^n} = 1$ .  $\square$

Using the Dirichlet-Jordan test, we can prove a slightly stronger form of the Poisson summation formula in the single variable setting for the complete integral lattice  $\mathbb{Z}$ .

**Theorem 3.2.** *Suppose  $f(x)$  is absolutely integrable on  $\mathbb{R}$ , and the function*

$$F(x) = \sum_{n \in \mathbb{Z}}^* f(x + n),$$

*satisfies the Dirichlet-Jordan test, where the  $*$  in the sum indicates that  $f(x + n)$  is meant to represent the average of the left-hand and right-hand limits at jump discontinuities. Then*

$$\sum_{n \in \mathbb{Z}}^* f(x + n) = \sum_{t \in \mathbb{Z}} (\mathcal{F}f)(t) e^{2\pi i t x},$$

*and*

$$\sum_{n \in \mathbb{Z}}^* f(n) = \sum_{t \in \mathbb{Z}} (\mathcal{F}f)(t).$$

*Proof.* Observe that  $F(x)$  is 1-periodic. As  $F(x)$  satisfies the Dirichlet-Jordan test by assumption, it admits a Fourier series converging locally uniformly to  $F(x)$  wherever  $F(x)$  is continuous. In fact, by the construction of  $F(x)$  and that the Fourier series of  $F(x)$  converges to the average of the left-hand and right-hand limits at jump discontinuities, the Fourier series of  $F(x)$  converges locally uniformly to  $F(x)$  everywhere. Moreover,  $F(x)$  is absolutely integrable on  $[0, 1]$ . We compute the  $t$ -th Fourier coefficient of  $F(x)$  given by

$$\hat{F}(t) = \int_0^1 F(x) e^{-2\pi i t x} dx.$$

The absolute integrability of  $f(x)$  permits the interchange of sum and integral to obtain

$$\int_{-\infty}^{\infty} f(x) e^{-2\pi i t x} dx = (\mathcal{F}f)(t).$$

Whence

$$\sum_{n \in \mathbb{Z}}^* f(x + n) = \sum_{t \in \mathbb{Z}} (\mathcal{F}f)(t) e^{2\pi i t x}.$$

This proves the first statement. Setting  $x = 0$  proves the second statement.  $\square$

In practical settings, we need a class of functions  $f(\mathbf{x})$  for which the assumptions of the Poisson summation formula hold. We say that  $f(\mathbf{x})$  is of *Schwarz class* if  $f \in C^\infty(\mathbb{R}^n)$  and  $f(\mathbf{x})$  along with all of its partial derivatives have rapid decay. If  $f(\mathbf{x})$  is of Schwarz class, the rapid decay implies that  $f(\mathbf{x})$  and all of its derivatives are absolutely integrable over  $\mathbb{R}^n$ . Moreover,  $F(\mathbf{x}) = \sum_{\mathbf{n} \in \mathbb{Z}^n} f(\mathbf{x} + \mathbf{n})$  and all of its derivatives are locally absolutely uniformly convergent by the Weierstrass  $M$ -test. The uniform limit theorem then ensures  $F(\mathbf{x})$  is smooth and thus the conditions of the Poisson summation formula are satisfied. So in most practical applications only needed to ensure that  $f(\mathbf{x})$  is Schwarz class.

We now introduce some explicit Schwarz class functions and compute their Fourier transforms. The classic example is  $e^{-2\pi x^2}$ . This function is particularly important because it is essentially its own Fourier transform.

**Proposition 3.3.** *Let  $\alpha > 0$  and set  $f(x) = e^{-2\pi\alpha x^2}$ . Then*

$$(\mathcal{F}f)(\zeta) = \frac{e^{-\frac{\pi\zeta^2}{2\alpha}}}{\sqrt{2\alpha}}.$$

*In particular,  $e^{-\pi x^2}$  is its own Fourier transform.*

*Proof.* Consider

$$(\mathcal{F}f)(\zeta) = \int_{-\infty}^{\infty} e^{-2\pi(\alpha x^2 + i\zeta x)} dx.$$

The change of variables  $x \mapsto \frac{x}{\sqrt{\alpha}}$  transforms this integral into

$$\frac{1}{\sqrt{\alpha}} \int_{-\infty}^{\infty} e^{-2\pi\left(x^2 + \frac{i\zeta x}{\sqrt{\alpha}}\right)} dx.$$

Complete the square in the exponent by observing

$$x^2 + \frac{i\zeta x}{\sqrt{\alpha}} = \left(x + \frac{i\zeta}{2\sqrt{\alpha}}\right)^2 + \frac{\zeta^2}{4\alpha},$$

so that the previous integral is equal to

$$\frac{e^{-\frac{\pi\zeta^2}{2\alpha}}}{\sqrt{\alpha}} \int_{-\infty}^{\infty} e^{-2\pi\left(x + \frac{i\zeta}{2\sqrt{\alpha}}\right)^2} dx.$$

By rapid decay of the integrand, the change of variables  $x \mapsto \frac{x}{\sqrt{2}} - \frac{i\zeta}{\sqrt{\alpha}}$  is permitted giving

$$\frac{e^{-\frac{\pi\zeta^2}{2\alpha}}}{\sqrt{2\alpha}} \int_{-\infty}^{\infty} e^{-\pi x^2} dx = \frac{e^{-\frac{\pi\zeta^2}{2\alpha}}}{\sqrt{2\alpha}},$$

because the remaining integral is the Gaussian integral. This proves the first statement. The second statement follows by taking  $\alpha = \frac{1}{2}$ .  $\square$

The analog of  $e^{-2\pi x^2}$  on  $\mathbb{R}^n$  is  $e^{-2\pi\langle \mathbf{x}, \mathbf{x} \rangle}$  which is Schwarz class because  $e^{-2\pi x^2}$  is. We also obtain a generalization of the previous result this Schwarz class function as a corollary.

**Corollary 3.4.** *Let  $\alpha > 0$  and set  $f(\mathbf{x}) = e^{-2\pi\alpha\langle \mathbf{x}, \mathbf{x} \rangle}$ . Then*

$$(\mathcal{F}f)(\boldsymbol{\xi}) = \frac{e^{-\frac{\pi\langle \boldsymbol{\xi}, \boldsymbol{\xi} \rangle}{2\alpha}}}{(2\alpha)^{\frac{n}{2}}}.$$

*In particular,  $e^{-\pi\langle \mathbf{x}, \mathbf{x} \rangle}$  is its own Fourier transform.*

*Proof.* Applying Proposition 3.3 to each variable separately proves the first statement. The second statement follows upon setting  $\alpha = \frac{1}{2}$ .  $\square$